## 牛顿一次迭代求Logistic解析解

$$
J(\theta)=\frac1m\sum_{i=1}^m\log(1+e^{-y^{(i)}\theta^Tx^{(i)}})=-\frac1m\sum_{i=1}^m\log(h_\theta(y^{(i)}x^{(i)}))
$$

- Solution:

$$
\begin{array}{l}
\nabla J(\theta)=-\frac1m\sum_{i=1}^my^{(i)}x^{(i)}(1-h_\theta(y^{(i)}x^{(i)})) \\
\begin{aligned}
H=\frac{\partial J}{\partial\theta\partial\theta^T}&=\frac{\partial J}{\partial\theta}(\frac1m\sum_{i=1}^my^{(i)}x^{(i)}h_\theta(y^{(i)}x^{(i)}))^T \\
&=\frac1m\sum_{i=1}^m{y^{(i)}}^2h_\theta(y^{(i)}x^{(i)})(1-h_\theta(y^{(i)}x^{(i)}))x^{(i)}{x^{(i)}}^T \\
&=\frac1m\sum_{i=1}^mh_\theta(y^{(i)}x^{(i)})(1-h_\theta(y^{(i)}x^{(i)}))x^{(i)}{x^{(i)}}^T
\end{aligned}
\end{array}
$$

- Iteration:

$$
x:=x-\frac{\nabla J(\theta)}{H}=x+\frac{\sum_{i=1}^my^{(i)}x^{(i)}(1-h_\theta(y^{(i)}x^{(i)}))}{\sum_{i=1}^mh_\theta(y^{(i)}x^{(i)})(1-h_\theta(y^{(i)}x^{(i)}))x^{(i)}{x^{(i)}}^T}
$$

